Bdd/Basic.lean
@@ -380,8 +380,42 @@ lemma OBdd.ordered_of_reachable {n m} {O : OBdd n m} {p} :
 lemma OBdd.ordered_of_relevant {n m} (O : OBdd n m) (S : O.1.RelevantPointer) :
     Ordered {heap := O.1.heap, root := S.1} := ordered_of_reachable S.2
 
-def OBdd.sub {n m} (O : OBdd n m) (p : O.bdd.RelevantPointer) : OBdd n m :=
+def OBdd.subBdd {n m} (O : OBdd n m) (p : O.bdd.RelevantPointer) : OBdd n m :=
   ⟨⟨O.bdd.heap, p⟩, O.ordered_of_reachable p.prop⟩
+
+lemma OBdd.subBdd_eq {n m} (O : OBdd n m) p :
+    O.subBdd p = ⟨⟨O.bdd.heap, p⟩, O.ordered_of_reachable p.prop⟩ := (rfl)
+
+@[simp]
+lemma OBdd.heap_subBdd {n m} {O : OBdd n m} p :
+    (O.subBdd p).bdd.heap = O.bdd.heap := (rfl)
+
+@[simp]
+lemma OBdd.root_subBdd {n m} {O : OBdd n m} p :
+    (O.subBdd p).bdd.root = p := (rfl)
+
+@[simp]
+lemma OBdd.subBdd_root {n m} (O : OBdd n m) : O.subBdd ⟨O.bdd.root, .refl⟩ = O := (rfl)
+
+lemma OBdd.reachable_low_of_subBdd {n m} {O : OBdd n m} {p j} (h : (O.subBdd p).bdd.root = node j) :
+    Reachable O.bdd.heap O.bdd.root O.bdd.heap[j].low := by
+  simp only [root_subBdd] at h
+  exact .snoc p.2 (h ▸ Edge.low)
+
+@[simp]
+lemma OBdd.low_subBdd {n m} {O : OBdd n m} {p} {j} {h : (O.subBdd p).bdd.root = node j} :
+    (O.subBdd p).low h = O.subBdd ⟨O.bdd.heap[j].low, reachable_low_of_subBdd h⟩ := by
+  simp only [subBdd_eq, eq_iff_bdd_eq, low_heap_eq_heap, low_root_eq_low, and_self]
+
+lemma OBdd.reachable_high_of_subBdd {n m} {O : OBdd n m} {p j} (h : (O.subBdd p).bdd.root = node j) :
+    Reachable O.bdd.heap O.bdd.root O.bdd.heap[j].high := by
+  simp only [root_subBdd] at h
+  exact .snoc p.2 (h ▸ Edge.high)
+
+@[simp]
+lemma OBdd.high_subBdd {n m} {O : OBdd n m} {p} {j} {h : (O.subBdd p).bdd.root = node j} :
+    (O.subBdd p).high h = O.subBdd ⟨O.bdd.heap[j].high, reachable_high_of_subBdd h⟩ := by
+  simp only [subBdd_eq, eq_iff_bdd_eq, high_heap_eq_heap, high_root_eq_high, and_self]
 
 /-! ## var -/
 
@@ -573,28 +607,36 @@ termination_by O
 
 /-! ## Similarity -/
 
-@[expose]
-def OBdd.HSimilar {n m m'} (O : OBdd n m) (U : OBdd n m') := O.toTree = U.toTree
+def OBdd.Similar {n m m'} (O : OBdd n m) (U : OBdd n m') := O.toTree = U.toTree
 
-def OBdd.Similar {n m} : OBdd n m → OBdd n m → Prop := HSimilar
+lemma OBdd.similar_iff {n m m'} {O : OBdd n m} {U : OBdd n m'} :
+    O.Similar U ↔ O.toTree = U.toTree := by rfl
 
-def OBdd.SimilarRP {n m} (O : OBdd n m) (p q : O.1.RelevantPointer) :=
-  Similar ⟨{heap := O.1.heap, root := p.1}, ordered_of_reachable p.2⟩
-          ⟨{heap := O.1.heap, root := q.1}, ordered_of_reachable q.2⟩
+lemma OBdd.similar_low {n m m'} {O : OBdd n m} {U : OBdd n m'}
+    {j} (h1 : O.bdd.root = .node j) {j'} (h2 : U.bdd.root = .node j') :
+    O.Similar U → (O.low h1).Similar (U.low h2):= by
+  grind only [similar_iff, toTree_node h1, toTree_node h2]
 
-lemma OBdd.similarRP_iff {n m} {O : OBdd n m} {p q : O.1.RelevantPointer} : O.SimilarRP p q ↔
-    (OBdd.mk ⟨O.bdd.heap, p⟩ (ordered_of_reachable p.2)).toTree =
-    (OBdd.mk ⟨O.bdd.heap, q⟩ (ordered_of_reachable q.2)).toTree := by rfl
+lemma OBdd.similar_high {n m m'} {O : OBdd n m} {U : OBdd n m'}
+    {j} (h1 : O.bdd.root = .node j) {j'} (h2 : U.bdd.root = .node j') :
+    O.Similar U → (O.high h1).Similar (U.high h2):= by
+  grind only [similar_iff, toTree_node h1, toTree_node h2]
+
+def OBdd.SimilarRP {n m m'} {O : OBdd n m} {U : OBdd n m'} p q :=
+  Similar (O.subBdd p) (U.subBdd q)
+
+lemma OBdd.similarRP_iff {n m m'} {O : OBdd n m} {U : OBdd n m'} {p q} :
+    O.SimilarRP p q ↔ (O.subBdd p).toTree = (U.subBdd q).toTree := by rfl
 
 /-- Isomorphism of `Ordered` BDDs is an equivalence relation. -/
 lemma OBdd.Similar.instEquivalence {n m} : Equivalence (α := OBdd n m) OBdd.Similar := by
   apply InvImage.equivalence
-  constructor <;> simp_all [HSimilar]
+  constructor <;> simp_all
 
-lemma OBdd.HSimilar_of_terminal {n m m' : Nat} {b : Bool} {O : OBdd n m} {U : OBdd n m'} :
-    O.1.root = terminal b → U.1.root = terminal b → O.HSimilar U := by
+lemma OBdd.Similar_of_terminal {n m m' : Nat} {b : Bool} {O : OBdd n m} {U : OBdd n m'} :
+    O.1.root = terminal b → U.1.root = terminal b → O.Similar U := by
   intro h1 h2
-  simp [HSimilar]
+  simp only [similar_iff]
   rw [toTree_terminal h1, toTree_terminal h2]
 
 /-! ## OBdd.Reduced -/
@@ -621,7 +663,7 @@ def OBdd.Reduced {n m} (O : OBdd n m) : Prop
   -- No redundant pointers.
   := NoRedundancy O.1
   -- Similarity implies pointer-equality.
-   ∧ Subrelation (SimilarRP O) (InvImage Eq Subtype.val)
+   ∧ Subrelation O.SimilarRP (InvImage Eq Subtype.val)
 
 /-- The graph induced by a terminal BDD consists of a sole terminal pointer. -/
 private lemma Bdd.terminal_relevant_iff {n m} {B : Bdd n m} {b} (h : B.root = terminal b)
@@ -653,30 +695,30 @@ lemma Bdd.reduced_of_terminal : OBdd.Reduced ⟨⟨M, terminal b⟩, o⟩ :=
   OBdd.reduced_of_terminal rfl
 
 /-- Sub-BDDs of a reduced BDD are reduced. -/
-private lemma OBdd.reduced_of_relevant {n m} {O : OBdd n m} (S : O.1.RelevantPointer):
-    O.Reduced → OBdd.Reduced ⟨{heap := O.1.heap, root := S.1}, ordered_of_relevant O S⟩ := by
+private lemma OBdd.reduced_subBdd {n m} {O : OBdd n m} (S : O.1.RelevantPointer):
+    O.Reduced → OBdd.Reduced (O.subBdd S) := by
   intro R
   induction O using OBdd.init_inductionOn
   case base b U h1 h2 =>
     apply OBdd.reduced_of_terminal
-    simp_rw [Bdd.eq_terminal_of_relevant h2 S]
+    simp_rw [root_subBdd, Bdd.eq_terminal_of_relevant h2 S]
     rfl
   case step O' _ _ _ _ _ =>
     constructor
     · intro p; apply R.1 ⟨p.1, Reachable.trans S.2 p.2⟩
     · intro q p _
       have : O'.SimilarRP ⟨q.1, Reachable.trans S.2 q.2⟩ ⟨p.1, Reachable.trans S.2 p.2⟩ := by
-        simp_all only [SimilarRP, Similar]
+        simp_all only [similarRP_iff, subBdd_eq]
       apply R.2 this
 
 lemma OBdd.high_reduced {n m} {O : OBdd n m} {j : Fin m} {h : O.1.root = node j} : O.Reduced → (O.high h).Reduced := by
   intro o
-  apply reduced_of_relevant ⟨O.1.heap[j].high, ?_⟩ o
+  apply reduced_subBdd ⟨O.1.heap[j].high, ?_⟩ o
   exact O.bdd.reachable_high h
 
 lemma OBdd.low_reduced {n m} {O : OBdd n m} {j : Fin m} {h : O.1.root = node j} : O.Reduced → (O.low h).Reduced := by
   intro o
-  apply reduced_of_relevant ⟨O.1.heap[j].low, ?_⟩ o
+  apply reduced_subBdd ⟨O.1.heap[j].low, ?_⟩ o
   exact O.bdd.reachable_low h
 
 /-! ## Size -/
@@ -779,19 +821,19 @@ private lemma OBdd.not_reduced_of_sim_high_low {n m} {O : OBdd n m} {j : Fin m} 
   simp [toRelevantPointer]
   rw [h]
   constructor
-  have giso : SimilarRP O ⟨(O.high h).1.root, O.bdd.reachable_high h⟩
+  have giso : SimilarRP ⟨(O.high h).1.root, O.bdd.reachable_high h⟩
                                 ⟨(O.low  h).1.root, O.bdd.reachable_low h⟩ := iso
   exact (symm (R.2 giso))
 
 /-- Reduced OBDDs are canonical.  -/
 theorem OBdd.Canonicity {n m m'} {O : OBdd n m} {U : OBdd n m'} (ho : O.Reduced) (hu : U.Reduced) :
-    O.evaluate = U.evaluate → O.HSimilar U := by
+    O.evaluate = U.evaluate → O.Similar U := by
   intro h
   cases O_root_def : O.1.root with
   | terminal b =>
     cases U_root_def : U.1.root with
     | terminal c =>
-      simp only [HSimilar]
+      simp only [similar_iff]
       simp [evaluate_terminal O_root_def, evaluate_terminal U_root_def] at h
       rw [toTree_terminal O_root_def]
       grind [evaluate_def, toTree_terminal]
@@ -826,7 +868,7 @@ theorem OBdd.Canonicity {n m m'} {O : OBdd n m} {U : OBdd n m'} (ho : O.Reduced)
       apply not_reduced_of_sim_high_low O_root_def
       apply OBdd.Canonicity (high_reduced ho) (low_reduced ho) this
     | node i =>
-      simp only [HSimilar]
+      simp only [similar_iff]
       rw [toTree_node O_root_def, toTree_node U_root_def]
       simp only [DecisionTree.branch.injEq]
       have same_var : O.1.heap[j].var = U.1.heap[i].var := by
@@ -843,7 +885,7 @@ theorem OBdd.Canonicity {n m m'} {O : OBdd n m} {U : OBdd n m'} (ho : O.Reduced)
           have that : OBdd.Similar (U.high U_root_def) (U.low U_root_def) :=
             OBdd.Canonicity (high_reduced hu) (low_reduced hu) (evaluate_high_eq_evaluate_low_of_independentOf_root this)
           constructor
-          have iso : SimilarRP U ⟨(U.high U_root_def).1.root, U.1.reachable_high U_root_def⟩
+          have iso : SimilarRP ⟨(U.high U_root_def).1.root, U.1.reachable_high U_root_def⟩
                                   ⟨(U.low  U_root_def).1.root, U.1.reachable_low U_root_def⟩ := that
           exact (symm (hu.2 iso))
         · intro contra
@@ -858,7 +900,7 @@ theorem OBdd.Canonicity {n m m'} {O : OBdd n m} {U : OBdd n m'} (ho : O.Reduced)
           simp [toRelevantPointer]
           rw [O_root_def]
           constructor
-          have iso : SimilarRP O ⟨(O.high O_root_def).1.root, O.1.reachable_high O_root_def⟩
+          have iso : SimilarRP ⟨(O.high O_root_def).1.root, O.1.reachable_high O_root_def⟩
                                   ⟨(O.low  O_root_def).1.root, O.1.reachable_low O_root_def⟩ := that
           exact (symm (ho.2 iso))
       constructor
@@ -873,9 +915,9 @@ decreasing_by
   all_goals
     simp [OBdd.size'_node O_root_def, OBdd.size'_node U_root_def]; omega
 
-theorem OBdd.Canonicity_reverse {O : OBdd n m} {U : OBdd n m'}:
-    O.HSimilar U → O.evaluate = U.evaluate := by
-  simp_all [evaluate, Function.comp_apply, HSimilar]
+theorem OBdd.Canonicity_reverse {n m m'} {O : OBdd n m} {U : OBdd n m'}:
+    O.Similar U → O.evaluate = U.evaluate := by
+  simp_all [evaluate, Function.comp_apply, similar_iff]
 
 /-! ## Lemmas about Ordered -/
 
