Bdd/Sim.lean
@@ -10,16 +10,78 @@ structure State {n m m'} (O : OBdd n m) (U : OBdd n m') where
   rl : Std.HashMap (Fin m') (Fin m)
   hl : ∀ j j',
     lr[j]? = some j' → rl[j']? = some j           ∧
-    Pointer.Reachable O.1.heap O.1.root (.node j) ∧
-    ∃ hj : Bdd.Ordered ⟨O.1.heap, .node j⟩,
-      ∃ hj' : Bdd.Ordered ⟨U.1.heap, .node j'⟩,
-        OBdd.HSimilar ⟨⟨O.1.heap, .node j⟩, hj⟩ ⟨⟨U.1.heap, .node j'⟩, hj'⟩
+    ∃ hj hj', OBdd.Similar (O.subBdd ⟨.node j, hj⟩) (U.subBdd ⟨.node j', hj'⟩)
   hr : ∀ j j',
     rl[j']? = some j → lr[j]? = some j'            ∧
-    Pointer.Reachable U.1.heap U.1.root (.node j') ∧
-    ∃ hj : Bdd.Ordered ⟨O.1.heap, .node j⟩,
-      ∃ hj' : Bdd.Ordered ⟨U.1.heap, .node j'⟩,
-        OBdd.HSimilar ⟨⟨O.1.heap, .node j⟩, hj⟩ ⟨⟨U.1.heap, .node j'⟩, hj'⟩
+    ∃ hj hj', OBdd.Similar (O.subBdd ⟨.node j, hj⟩) (U.subBdd ⟨.node j', hj'⟩)
+
+def State.insert {n m m'} {O : OBdd n m} {U : OBdd n m'} (s : State O U) (j : Fin m) (j' : Fin m')
+    (hrj : Pointer.Reachable O.bdd.heap O.bdd.root (Pointer.node j))
+    (hrj' : Pointer.Reachable U.bdd.heap U.bdd.root (Pointer.node j'))
+    (hv : O.bdd.heap[j].var = U.bdd.heap[j'].var)
+    (hl : s.lr[j]? = none)
+    (hr : s.rl[j']? = none)
+    (h : (O.subBdd ⟨O.bdd.heap[j].low, .snoc hrj Edge.low⟩).Similar
+      (U.subBdd ⟨U.bdd.heap[j'].low, .snoc hrj' Edge.low⟩))
+    (h' : (O.subBdd ⟨O.bdd.heap[j].high, .snoc hrj Edge.high⟩).Similar
+      (U.subBdd ⟨U.bdd.heap[j'].high, .snoc hrj' Edge.high⟩))
+    : State O U where
+  lr := s.lr.insert j j'
+  rl := s.rl.insert j' j
+  hl jj jj' hjj := by
+    simp only [Std.HashMap.getElem?_insert, beq_iff_eq] at hjj
+    split at hjj
+    next heq =>
+      subst heq
+      simp only [Std.HashMap.getElem?_insert, beq_iff_eq]
+      split
+      next heqq =>
+        subst heqq
+        simp only [true_and]
+        use hrj, hrj'
+        simp only [OBdd.similar_iff] at ⊢ h h'
+        rw [OBdd.toTree_node (OBdd.root_subBdd ⟨.node j, _⟩)]
+        rw [OBdd.toTree_node (OBdd.root_subBdd ⟨.node j', _⟩)]
+        simp only [OBdd.heap_subBdd, OBdd.low_subBdd, OBdd.high_subBdd,
+          DecisionTree.branch.injEq]
+        exact ⟨hv, h, h'⟩
+      next heqq => injection hjj; contradiction
+    next heq =>
+      simp only [Std.HashMap.getElem?_insert, beq_iff_eq]
+      split
+      next heqq =>
+        subst heqq
+        rw [(s.hl jj j' hjj).1] at hr
+        contradiction
+      next heqq =>
+        exact s.hl jj jj' hjj
+  hr jj jj' hjj := by
+    simp only [Std.HashMap.getElem?_insert, beq_iff_eq] at hjj
+    split at hjj
+    next heq =>
+      subst heq
+      simp only [Std.HashMap.getElem?_insert, beq_iff_eq]
+      split
+      next heqq =>
+        subst heqq
+        simp only [true_and]
+        use hrj, hrj'
+        simp only [OBdd.similar_iff] at ⊢ h h'
+        rw [OBdd.toTree_node (OBdd.root_subBdd ⟨.node j, _⟩)]
+        rw [OBdd.toTree_node (OBdd.root_subBdd ⟨.node j', _⟩)]
+        simp only [OBdd.heap_subBdd, OBdd.low_subBdd, OBdd.high_subBdd,
+          DecisionTree.branch.injEq]
+        exact ⟨hv, h, h'⟩
+      next heqq => injection hjj; contradiction
+    next heq =>
+      simp only [Std.HashMap.getElem?_insert, beq_iff_eq]
+      split
+      next heqq =>
+        subst heqq
+        rw [(s.hr j jj' hjj).1] at hl
+        contradiction
+      next heqq =>
+        exact s.hr jj jj' hjj
 
 def sim_helper {n m m'}
     (O : OBdd n m) (hO : OBdd.Reduced O)
@@ -28,21 +90,20 @@ def sim_helper {n m m'}
     (q : Pointer m') (hqr : Pointer.Reachable U.1.heap U.1.root q) :
   StateM
     (State O U)
-    (Decidable
-      (OBdd.HSimilar
-        ⟨⟨O.1.heap, p⟩, O.ordered_of_reachable hpr⟩
-        ⟨⟨U.1.heap, q⟩, U.ordered_of_reachable hqr⟩)) :=
+    (Decidable (OBdd.Similar (O.subBdd ⟨p, hpr⟩) (U.subBdd ⟨q, hqr⟩))) :=
   match hp : p with
   | .terminal b =>
     match hq : q with
     | .terminal b' =>
       if hb : b = b'
-      then return isTrue (by simpa [OBdd.HSimilar, OBdd.toTree_terminal])
-      else return isFalse (by simpa [OBdd.HSimilar, OBdd.toTree_terminal])
-    | .node j' => return isFalse (by simp [OBdd.HSimilar, OBdd.toTree_terminal, OBdd.toTree_node])
+      then return isTrue <| by simpa [OBdd.similar_iff, OBdd.toTree_terminal]
+      else return isFalse <| by simpa [OBdd.similar_iff, OBdd.toTree_terminal]
+    | .node j' =>
+      return isFalse <| by simp [OBdd.similar_iff, OBdd.toTree_terminal, OBdd.toTree_node]
   | .node j =>
     match hq : q with
-    | .terminal b' => return isFalse (by simp [OBdd.HSimilar, OBdd.toTree_terminal, OBdd.toTree_node])
+    | .terminal b' =>
+      return isFalse <| by simp [OBdd.similar_iff, OBdd.toTree_terminal, OBdd.toTree_node]
     | .node j' =>
       if hv : O.1.heap[j].var = U.1.heap[j'].var
       then do
@@ -52,124 +113,63 @@ def sim_helper {n m m'}
           match hr : s.rl[j']? with
           | none =>
             let hll ← sim_helper O hO U hU
-              O.1.heap[j].low (Pointer.Reachable.snoc hpr .low)
-              U.1.heap[j'].low (Pointer.Reachable.snoc hqr .low)
-            match hll with
-            | isTrue ht =>
-              -- TODO : why is type declaration needed? Note that only `←` does not work, for some reason `:= ←` is needed
-              let hhh : Decidable (OBdd.HSimilar ⟨Bdd.mk O.bdd.heap O.bdd.heap[j].high, _⟩ ⟨Bdd.mk U.bdd.heap U.bdd.heap[j'].high, _⟩) :=
+              O.1.heap[j].low (.snoc hpr .low) U.1.heap[j'].low (.snoc hqr .low)
+            if h : (O.subBdd ⟨O.bdd.heap[j].low, _⟩).Similar (U.subBdd ⟨U.bdd.heap[j'].low, _⟩) then
+              let hhh :=
                 ← sim_helper O hO U hU
                 O.1.heap[j].high (Pointer.Reachable.snoc hpr .high)
                 U.1.heap[j'].high (Pointer.Reachable.snoc hqr .high)
-              match hhh with
-              | isTrue ht' =>
-                set
-                  (⟨s.lr.insert j j', s.rl.insert j' j,
-                    fun jj jj' hjj ↦ by
-                      simp only [Std.HashMap.getElem?_insert, beq_iff_eq] at hjj
-                      split at hjj
-                      next heq =>
-                        subst heq
-                        simp only [Std.HashMap.getElem?_insert, beq_iff_eq]
-                        split
-                        next heqq =>
-                          subst heqq
-                          simp only [true_and]
-                          constructor
-                          · exact hpr
-                          · use OBdd.ordered_of_reachable hpr
-                            use OBdd.ordered_of_reachable hqr
-                            simp only [OBdd.HSimilar] at ⊢ ht ht'
-                            rw [OBdd.toTree_node rfl, OBdd.toTree_node (j := j') rfl]
-                            simp only [OBdd.low_eq, Bdd.low_eq, OBdd.high_eq, Bdd.high_eq,
-                              DecisionTree.branch.injEq]
-                            exact ⟨hv, ht, ht'⟩
-                        next heqq => injection hjj; contradiction
-                      next heq =>
-                        simp only [Std.HashMap.getElem?_insert, beq_iff_eq]
-                        split
-                        next heqq =>
-                          subst heqq
-                          rw [(s.hl jj j' hjj).1] at hr
-                          contradiction
-                        next heqq =>
-                          exact s.hl jj jj' hjj,
-                    fun jj jj' hjj ↦ by
-                      simp only [Std.HashMap.getElem?_insert, beq_iff_eq] at hjj
-                      split at hjj
-                      next heq =>
-                        subst heq
-                        simp only [Std.HashMap.getElem?_insert, beq_iff_eq]
-                        split
-                        next heqq =>
-                          subst heqq
-                          simp only [true_and]
-                          constructor
-                          · exact hqr
-                          · use OBdd.ordered_of_reachable hpr
-                            use OBdd.ordered_of_reachable hqr
-                            simp only [OBdd.HSimilar] at ⊢ ht ht'
-                            rw [OBdd.toTree_node rfl, OBdd.toTree_node (j := j') rfl]
-                            simp only [OBdd.low_eq, Bdd.low_eq, OBdd.high_eq, Bdd.high_eq,
-                              DecisionTree.branch.injEq]
-                            exact ⟨hv, ht, ht'⟩
-                        next heqq => injection hjj; contradiction
-                      next heq =>
-                        simp only [Std.HashMap.getElem?_insert, beq_iff_eq]
-                        split
-                        next heqq =>
-                          subst heqq
-                          rw [(s.hr j jj' hjj).1] at hl
-                          contradiction
-                        next heqq =>
-                          exact s.hr jj jj' hjj
-                   ⟩ : State O U)
-                return isTrue (by
-                  simp only [OBdd.HSimilar] at ⊢ ht ht'
-                  rw [OBdd.toTree_node rfl, OBdd.toTree_node (j := j') rfl]
-                  simp only [OBdd.low_eq, Bdd.low_eq, OBdd.high_eq, Bdd.high_eq,
+              if h' : (O.subBdd ⟨O.bdd.heap[j].high, _⟩).Similar (U.subBdd ⟨U.bdd.heap[j'].high, _⟩) then
+                set (s.insert j j' hpr hqr hv hl hr h h')
+                return isTrue <| by
+                  simp only [OBdd.similar_iff] at ⊢ h h'
+                  rw [OBdd.toTree_node (OBdd.root_subBdd ⟨.node j, _⟩)]
+                  rw [OBdd.toTree_node (OBdd.root_subBdd ⟨.node j', _⟩)]
+                  simp only [OBdd.heap_subBdd, OBdd.low_subBdd, OBdd.high_subBdd,
                     DecisionTree.branch.injEq]
-                  exact ⟨hv, ht, ht'⟩
-                )
-              | isFalse hf' => return isFalse (fun c ↦ by
-                simp [OBdd.HSimilar, OBdd.toTree_node, OBdd.high_eq, Bdd.high_eq] at c;
-                exact hf' c.2.2)
-            | isFalse hf => return isFalse (fun c ↦ by
-              simp [OBdd.HSimilar, OBdd.toTree_node, OBdd.low_eq, Bdd.low_eq] at c; exact hf c.2.1)
+                  exact ⟨hv, h, h'⟩
+              else
+                return isFalse <| by
+                  intro c
+                  have := OBdd.similar_high (OBdd.root_subBdd _) (OBdd.root_subBdd _) c
+                  grind only [OBdd.high_subBdd]
+            else
+              return isFalse <| by
+                intro c
+                have := OBdd.similar_low (OBdd.root_subBdd _) (OBdd.root_subBdd _) c
+                grind only [OBdd.low_subBdd]
           | some i =>
-            return isFalse (by
-              rcases s.hr i j' hr with ⟨h1, h2, h3, h4, h5⟩
-              rcases s.hl i j' h1 with ⟨h1', h2', h3', h4', h5'⟩
+            return isFalse <| by
+              rcases s.hr i j' hr with ⟨h1, h2, h3, h4⟩
+              rcases s.hl i j' h1 with ⟨h1', h2', h3', h4'⟩
               intro contra
-              have hsim : OBdd.SimilarRP O ⟨.node i, h2'⟩ ⟨.node j, hpr⟩ := by
-                simp [OBdd.similarRP_iff]
-                simp only [OBdd.HSimilar] at contra h5
-                rw [contra]
-                exact h5
+              have hsim : OBdd.SimilarRP ⟨.node i, h2'⟩ ⟨.node j, hpr⟩ := by
+                rw [OBdd.similar_iff] at contra h4
+                rw [OBdd.similarRP_iff, contra]
+                exact h4
               have h := hO.2 hsim
               simp [InvImage] at h
               subst h
               rw [h1] at hl
               contradiction
-            )
         | some i' =>
           if heq : j' = i'
           then
-            return isTrue (s.hl j j' (by simp_all)).2.2.2.2
+            return isTrue (s.hl j j' (by simp_all)).2.2.2
           else
-            return isFalse (fun c ↦ heq (by
-              rcases s.hl j i' hl with ⟨h1, h2, h3, h4, h5⟩
-              rcases s.hr j i' h1 with ⟨h1', h2', h3', h4', h5'⟩
-              have hsim : OBdd.SimilarRP U ⟨.node j', hqr⟩ ⟨.node i', h2'⟩ := by
-                simp [OBdd.similarRP_iff]
-                simp only [OBdd.HSimilar] at c h5
-                rw [c] at h5
-                exact h5
+            return isFalse <| by
+              intro c
+              rcases s.hl j i' hl with ⟨h1, h2, h3, h4⟩
+              rcases s.hr j i' h1 with ⟨h1', h2', h3', h4'⟩
+              have hsim : OBdd.SimilarRP ⟨.node j', hqr⟩ ⟨.node i', h3'⟩ := by
+                rw [OBdd.similarRP_iff]
+                rw [OBdd.similar_iff] at c h4
+                rw [c] at h4
+                exact h4
               have := hU.2 hsim
               simp [InvImage] at this
-              exact this
-            ))
-      else return isFalse (by simp_all [OBdd.HSimilar, OBdd.toTree_node])
+              exact heq this
+      else return isFalse <| by simp_all [OBdd.similar_iff, OBdd.toTree_node]
 termination_by OBdd.size' ⟨⟨O.1.heap, p⟩, O.ordered_of_reachable hpr⟩
 decreasing_by
   · simp [OBdd.size'_node, OBdd.low_eq, Bdd.low_eq]; omega
@@ -178,13 +178,8 @@ decreasing_by
 public def decidableRobddHSimilar {n m m'}
     (O : OBdd n m) (hO : O.Reduced)
     (U : OBdd n m') (hU : U.Reduced) :
-    Decidable (O.HSimilar U) :=
-  ((sim_helper O hO U hU O.1.root .refl U.1.root .refl)
-    ⟨ Std.HashMap.emptyWithCapacity 0,
-      Std.HashMap.emptyWithCapacity 0,
-      by simp,
-      by simp
-    ⟩
-  ).1
+    Decidable (O.Similar U) :=
+  O.subBdd_root ▸ U.subBdd_root ▸
+    (sim_helper O hO U hU O.1.root .refl U.1.root .refl ⟨∅, ∅, by simp, by simp⟩).1
 
 end Sim
